Tiny

coq-osiris/theories/program_logic/pure/spec_rules.v
@@ -49,33 +49,33 @@ Qed.
 
 (* -------------------------------------------------------------------------- *)
 
-(* As an example, we define [Spec'] as a way to specify unary functions. *)
+(* As an example, we define [Spec_Unary'] as a way to spec_unaryify unary functions. *)
 
-(* [call_spec] is the type of specifications over function calls. It
+(* [call_spec_unary] is the type of spec_unaryifications over function calls. It
   depends on two arguments: the argument of the function call, and the
   computation resulting from calling the function on that argument. *)
 
-Local Definition call_spec {A : Type} := A -> microvx -> Prop.
+Local Definition call_spec_unary {A : Type} := A -> microvx -> Prop.
 
-(* [Spec c P] states that given a closure [c], the specification [P]
+(* [Spec_Unary c P] states that given a closure [c], the spec_unaryification [P]
   holds for any call of [c] on an argument. *)
 
-Local Definition Spec `{Encode X} (c : val) (P : call_spec) :=
+Local Definition Spec_Unary `{Encode X} (c : val) (P : call_spec_unary) :=
   ∀ (x : X), P x (call c #x).
 
-(* Consider for example the specification of a function [sort]:
-  [ Spec sort (λ l m, pure m (λ l', Sorted l' ∧ l' ≡ l) ⊥) ] *)
+(* Consider for example the spec_unaryification of a function [sort]:
+  [ Spec_Unary sort (λ l m, pure m (λ l', Sorted l' ∧ l' ≡ l) ⊥) ] *)
 
-(* Example of a reasoning rule, for the creation of a [Spec c P]. *)
+(* Example of a reasoning rule, for the creation of a [Spec_Unary c P]. *)
 
-Local Lemma pure_eval_anon `{Encode X} (P : call_spec) η (xvar : var) e ζ :
+Local Lemma pure_eval_anon `{Encode X} (P : call_spec_unary) η (xvar : var) e ζ :
   (∀ (x : X),
       P x (eval ((xvar, #x) :: η) e)) ->
-  pure (eval η (EAnonFun (AnonFun xvar e))) (λ c, Spec c P) ζ.
+  pure (eval η (EAnonFun (AnonFun xvar e))) (λ c, Spec_Unary c P) ζ.
 Proof. intros; simpl_eval; by eapply pure_ret; eauto. Qed.
 
 (* [pure_eval_letrec] allows us to prove that the body [e] of a letrec
-  expression satisfies a specification given by [P].
+  expression satisfies a spec_unaryification given by [P].
 
   In a first subgoal, we prove that any function call satisfies [P],
   under the assumption that calls to smaller arguments (according to
@@ -83,26 +83,26 @@ Proof. intros; simpl_eval; by eapply pure_ret; eauto. Qed.
   In the second subgoal, we prove [e2] while abstracting over [e]. *)
 
 Local Lemma pure_eval_letrec `{Encode X, Encode Y}
-  (P : call_spec) (R : X -> X -> Prop) η f (x : var) e
+  (P : call_spec_unary) η f (x : var) e
   e2 (φ : Y -> Prop) ζ
   (* Show that the relation on which arguments are decreasing is well-founded. *)
-  {WF_x : WellFoundedRel _ R} :
-  (* Show the specification [P] holds over a call to any argument
+  {WF_x : WellFounded X} :
+  (* Show the spec_unaryification [P] holds over a call to any argument
     [arg], under the assumption that [P] holds to a call over any
     argument [yval] smaller than [arg]. *)
   (∀ c (arg : X),
-      Spec c (λ yval m, R yval arg -> P yval m) ->
+      Spec_Unary c (λ yval m, wf_relation (WF := WF_x) yval arg -> P yval m) ->
       P arg (eval ((x, #arg) :: (f, c) :: η) e)) ->
-  (* Continue with [f] bound to [c], and [c] specified by [P]. *)
-  (∀ c, Spec c P -> pure (eval ((f, c) :: η) e2) φ ζ) ->
+  (* Continue with [f] bound to [c], and [c] spec_unaryified by [P]. *)
+  (∀ c, Spec_Unary c P -> pure (eval ((f, c) :: η) e2) φ ζ) ->
   (* When facing an expression of the form [let rec f x = e in e2]. *)
   pure (eval η (ELetRec [RecBinding f (AnonFun x e)] e2)) φ ζ.
 Proof.
-  intros Hmkspec He2. simpl_eval. eapply He2.
-  unfold Spec. intros v.
-  induction v as [v IH] using (well_founded_induction Hwf); intros.
+  intros Hmkspec_unary He2. simpl_eval. eapply He2.
+  unfold Spec_Unary. intros v.
+  induction v as [v IH] using (well_founded_induction wf_def); intros.
   simpl; rewrite String.eqb_refl; simpl.
-  eapply Hmkspec. intros y. intros HR. by apply IH.
+  eapply Hmkspec_unary. intros y. intros HR. by apply IH.
 Qed.
 
 (* -------------------------------------------------------------------------- *)
@@ -110,27 +110,26 @@ Qed.
 From Equations Require Import Equations.
 
 (* We want to be able to reason on n-ary functions. We thus generalize
-   [Spec'] to take a list of arguments described by an [arg_type]. *)
+   [Spec] to take a list of arguments described by an [arg_type]. *)
 
 (* [Spec] matches on the list of argument types [arg_τ], producing a
    series of nested calls, where the base case is identical to the
-   definition of [Spec']. *)
+   definition of [Spec_Unary]. *)
 
-(* [Spec arg_τ c P] should be read as "[c] is a function value, with
-   arguments described by [arg_τ], and with specification [P]." *)
+(* [Spec args c P] should be read as "[c] is a function value, with
+   arguments described by [args], and with specification [P]." *)
 
-Equations Spec (arg_τ : arg_type)
-  (c : val) (P : arg_τ -#> microvx -> Prop) : Prop :=
-| Arg1 X, c, P :=
+Equations Spec (args : types) (c : val) (P : args -#> microvx -> Prop) : Prop :=
+| Tbase X, c, P :=
     ∀ (x : X), P x (call c #x)
-| ArgS X TT, c, P :=
+| Tcons X TT, c, P :=
     ∀ (x : X), pure_wp (call c #x) (λ c, Spec TT c (P x)) ⊥.
 
-Arguments Spec {arg_τ} c P.
+Arguments Spec {args} c P.
 
 (* We can check on a simple example that [Spec] generalizes [Spec']. *)
 
-Local Lemma pure_eval_anon_single `{Encode X} (P : tele[X] -#> microvx -> Prop) η (x : var) e ζ :
+Local Lemma pure_eval_anon_single `{Encode X} (P : τ[X] -#> microvx -> Prop) η (x : var) e ζ :
   (∀ (v : X), P v (eval ((x, #v) :: η) e)) ->
   pure (eval η (EAnonFun (AnonFun x e))) (λ c, Spec c P) ζ.
 Proof.
@@ -139,13 +138,13 @@ Qed.
 
 (* [Spec_mono] states that [Spec] is monotonic over specifications. *)
 
-Lemma Spec_mono (arg_τ : arg_type) (P P' : arg_τ -#> microvx -> Prop) c :
+Lemma Spec_mono (args : types) (P P' : args -#> microvx -> Prop) c :
   Spec c P ->
   (∀# args, ∀ m, (P args) m -> (P' args) m) ->
   Spec c P'.
 Proof.
   revert c.
-  induction arg_τ as [ | X HX arg_τ IH ]; intros c HP Hmono.
+  induction args as [ | X HX arg_τ IH ]; intros c HP Hmono.
   { simp Spec in HP |-*. intros x.
     apply Hmono. apply HP. }
   simp Spec in HP |-*; intros x.
